feat: udiv/umod bitblasting for LeanSAT

src/Init/Data/BitVec/Bitblast.lean
@@ -430,6 +430,394 @@ theorem shiftLeft_eq_shiftLeftRec (x : BitVec w₁) (y : BitVec w₂) :
   · simp [of_length_zero]
   · simp [shiftLeftRec_eq]
 
+/-! # udiv/urem recurrence for bitblasting
+
+In order to prove the correctness of the division algorithm on the integers,
+one shows that `n.div d = q` and `n.mod d = r` iff `n = d * q + r` and `0 ≤ r < d`.
+Mnemonic: `n` is the numerator, `d` is the denominator, `q` is the quotient, and `r` the remainder.
+
+This uniqueness property is not true for bitvectors.
+Let us study an instructive counterexample:
+
+- Let `bitwidth = 3`
+- Let `n = 0, d = 3`
+- If we choose `q = 2, r = 2`, then `d * q + r = 6 + 2 = 8 ≃ 0 (mod 8)` and (`r < d`).
+- But see that `q = 0, r = 0` also satisfies the constraints, as `0 * 3 + 0 = 0`.
+- So for (`n = 0, d = 3`), both (a) `q = 2, r = 2` as well as (b) `q = 0, r = 0` are solutions!
+
+Such examples can be created by choosing `(q, r)` for a fixed `(d, n)`
+such that `(d * q + r)` overflows and wraps around to equal `n`.
+
+This tells us that the division algorithm must have more restrictions that just the ones
+we have for natural numbers. These restrictions are captured in `DivModState.Lawful`,
+which captures the relationship necessary between `n, d, q, r`. The key idea is to state
+the relationship in terms of the `{n, d, q, r}.toNat` values, which implies that the
+relationship also holds at the bitvector level.
+
+References:
+- Fast 32-bit Division on the DSP56800E: Minimized nonrestoring division algorithm by David Baca
+- Bitwuzla sources for bitblasting.h
+-/
+
+private theorem Nat.div_add_eq_left_of_lt {x y z : Nat} (hx : z ∣ x) (hy : y < z) (hz : 0 < z) :
+    (x + y) / z = x / z := by
+  refine Nat.div_eq_of_lt_le ?lo ?hi
+  · apply Nat.le_trans
+    · exact div_mul_le_self x z
+    · omega
+  · simp only [succ_eq_add_one, Nat.add_mul, Nat.one_mul]
+    apply Nat.add_lt_add_of_le_of_lt
+    · apply Nat.le_of_eq
+      exact (Nat.div_eq_iff_eq_mul_left hz hx).mp rfl
+    · exact hy
+
+/-- If the division equation `d.toNat * q.toNat + r.toNat = n.toNat` holds,
+then `n.udiv d = q`. -/
+theorem udiv_eq_of_mul_add_toNat {d n q r : BitVec w} (hd : 0 < d)
+    (hrd : r < d)
+    (hdqnr : d.toNat * q.toNat + r.toNat = n.toNat) :
+    n.udiv d = q := by
+  apply BitVec.eq_of_toNat_eq
+  rw [toNat_udiv]
+  replace hdqnr : (d.toNat * q.toNat + r.toNat) / d.toNat = n.toNat / d.toNat := by
+    simp [hdqnr]
+  rw [Nat.div_add_eq_left_of_lt] at hdqnr
+  · rw [← hdqnr]
+    exact mul_div_right q.toNat hd
+  · exact Nat.dvd_mul_right d.toNat q.toNat
+  · exact hrd
+  · exact hd
+
+/-- If the division equation `d.toNat * q.toNat + r.toNat = n.toNat` holds,
+then `n.umod d = r` -/
+theorem umod_eq_of_mul_add_toNat {d n q r : BitVec w} (hrd : r < d)
+    (hdqnr : d.toNat * q.toNat + r.toNat = n.toNat) :
+    n.umod d = r := by
+  apply BitVec.eq_of_toNat_eq
+  rw [toNat_umod]
+  replace hdqnr : (d.toNat * q.toNat + r.toNat) % d.toNat = n.toNat % d.toNat := by
+    simp [hdqnr]
+  rw [Nat.add_mod, Nat.mul_mod_right] at hdqnr
+  simp only [Nat.zero_add, mod_mod] at hdqnr
+  replace hrd : r.toNat < d.toNat := by
+    simpa [BitVec.lt_def] using hrd
+  rw [Nat.mod_eq_of_lt hrd] at hdqnr
+  simp [hdqnr]
+
+/-! ### DivModState -/
+
+/-- Structure that maintains the state of recursive `divrem` calls. -/
+structure DivModState (w : Nat) : Type where
+  /-- The current quotient. -/
+  q : BitVec w
+  /-- The current remainder. -/
+  r : BitVec w
+
+/-- A `DivModState` is lawful if the remainder width `wr` plus the dividend width `wn` equals `w`,
+and the bitvectors `r` and `n` have values in the bounds given by bitwidths `wr`, resp. `wn`.
+
+This is a proof engineering choice: An alternative world could have
+`r : BitVec wr` and `n : BitVec wn`, but this required much more dependent typing coercions.
+
+Instead, we choose to declare all involved bitvectors as length `w`, and then prove that
+the values are within their respective bounds.
+-/
+structure DivModState.Lawful (w wr wn : Nat) (n d : BitVec w)
+    (qr : DivModState w) : Prop where
+  /-- The sum of widths of the dividend and remainder is `w`. -/
+  hwrn : wr + wn = w
+  /-- The divisor is positive. -/
+  hdPos : 0 < d
+  /-- The remainder is strictly less than the divisor. -/
+  hrLtDivisor : qr.r.toNat < d.toNat
+  /-- The remainder is morally a `Bitvec wr`, and so has value less than `2^wr`. -/
+  hrWidth : qr.r.toNat < 2^wr
+  /-- The quotient is morally a `Bitvec wr`, and so has value less than `2^wr`. -/
+  hqWidth : qr.q.toNat < 2^wr
+  /-- The low n bits of `n` obey the fundamental division equation. -/
+  hdiv : n.toNat >>> wn = d.toNat * qr.q.toNat + qr.r.toNat
+
+/-- A lawful DivModState implies `w > 0`. -/
+def DivModState.Lawful.hw {qr : DivModState w}
+    {h : DivModState.Lawful w wr wn n d qr} : 0 < w := by
+  have hd := h.hdPos
+  rcases w with rfl | w
+  · have hcontra : d = 0#0 := by apply Subsingleton.elim
+    rw [hcontra] at hd
+    simp at hd
+  · omega
+
+/-- An initial value with both `q, r = 0`. -/
+def DivModState.init (w : Nat) : DivModState w := {
+  q := 0#w
+  r := 0#w
+}
+
+/-- The initial state. -/
+def DivModState.Lawful.init (w : Nat) (n d : BitVec w) (hd : 0#w < d) :
+    DivModState.Lawful w 0 w n d (DivModState.init w) := {
+  hwrn := by omega,
+  hdPos := by assumption
+  hrLtDivisor := by simp [BitVec.lt_def] at hd ⊢; assumption
+  hrWidth := by simp [DivModState.init],
+  hqWidth := by simp [DivModState.init],
+  hdiv := by
+    simp only [DivModState.init, toNat_ofNat, zero_mod, Nat.mul_zero, Nat.add_zero];
+    rw [Nat.shiftRight_eq_div_pow]
+    apply Nat.div_eq_of_lt n.isLt
+}
+
+/--
+A lawful DivModState with a fully consumed dividend (`wn = 0`) witneses that the
+quotient has been correctly computed.
+-/
+theorem DivModState.udiv_eq_of_lawful_zero {qr : DivModState w}
+    (h : DivModState.Lawful w w 0 n d qr) :
+    n.udiv d = qr.q := by
+  apply udiv_eq_of_mul_add_toNat h.hdPos h.hrLtDivisor
+  have hdiv := h.hdiv
+  omega
+
+/--
+A lawful DivModState with a fully consumed dividend (`wn = 0`) witneses that the
+remainder has been correctly computed.
+-/
+theorem DivModState.umod_eq_of_lawful_zero {qr : DivModState w}
+    (h : DivModState.Lawful w w 0 n d qr) :
+    n.umod d = qr.r := by
+  apply umod_eq_of_mul_add_toNat h.hrLtDivisor
+  have hdiv := h.hdiv
+  simp only [shiftRight_zero] at hdiv
+  exact hdiv.symm
+
+/-! ### LawfulShiftSubtract -/
+
+/--
+A `LawfulShiftSubtract` is a `Lawful` DivModState that is also a legal input to the shift subtractor.
+So in particular, we must have at least one dividend bit left over `(0 < wn)`
+to perform a round of shift subtraction.
+
+The input to the shift subtractor is a legal input to `divrem`, and we also need to have an
+input bit to perform shift subtraction on, and thus we need `0 < wn`.
+-/
+structure DivModState.LawfulShiftSubtract (w wr wn : Nat) (n d : BitVec w) (qr : DivModState w)
+  extends DivModState.Lawful w wr wn n d qr : Type where
+  /-- Only perform a round of shift-subtract if we have dividend bits. -/
+  hwn_lt : 0 < wn
+
+/--
+In the shift subtract input, the dividend is at least one bit long (`wn > 0`), so
+the remainder has bits to be computed (`wr < w`).
+-/
+def DivModState.wr_lt_w {qr : DivModState w} (h : qr.LawfulShiftSubtract wr wn n d) : wr < w := by
+  have hwrn := h.hwrn
+  have hwn_lt := h.hwn_lt
+  omega
+
+/-- If we have extra bits to spare in `n`,
+then the div rem input can be converted into a shift subtract input
+to run a round of the shift subtracter. -/
+def DivModState.Lawful.toLawfulShiftSubtract {qr : DivModState w}
+    (h : qr.Lawful w wr (wn + 1) n d) : qr.LawfulShiftSubtract wr (wn + 1) n d where
+  hwrn := by have := h.hwrn; omega
+  hdPos := h.hdPos
+  hrLtDivisor := h.hrLtDivisor
+  hrWidth := h.hrWidth
+  hqWidth := h.hqWidth
+  hdiv := h.hdiv
+  hwn_lt := by omega
+
+/-! ### shiftConcat -/
+
+/--
+If `n : Bitvec w` has only the low `k < w` bits set,
+then `(n <<< 1 | b)` does not overflow.
+-/
+private theorem mul_two_add_lt_two_pow_of_lt_two_pow_of_lt_two {n b k w : Nat}
+    (hn : n < 2 ^ k) (hb : b < 2) (hk : k < w) :
+    n * 2 + b < 2 ^ w := by
+  have : 2^(k + 1) ≤ 2 ^w := Nat.pow_le_pow_of_le_right (by decide) (by assumption)
+  omega
+
+@[simp, bv_toNat]
+theorem toNat_shiftConcat {x : BitVec w} {b : Bool} : (x.shiftConcat b).toNat =
+    (x.toNat <<< 1 + b.toNat) % 2 ^ w  := by
+  simp only [shiftConcat]
+  rw [← add_eq_or_of_and_eq_zero] -- Due to `add_eq_or_of_and_eq_zero`, this must live in `Bitblast`.
+  · simp
+  · ext i
+    simp
+    omega
+
+/-- `x.shiftConcat b` does not overflow if `x < 2^k` for `k < w`, and so
+`x.shiftConcat b |>.toNat = x.toNat * 2 + b.toNat`. -/
+theorem toNat_shiftConcat_eq_of_lt_of_lt_two_pow {x : BitVec w} {b : Bool} {k : Nat}
+  (hk : k < w) (hx : x.toNat < 2 ^ k) :
+    (x.shiftConcat b).toNat = x.toNat * 2 + b.toNat := by
+  simp [bv_toNat, Nat.shiftLeft_eq]
+  have h := @Nat.pow_lt_pow_of_lt 2 k w (by omega) (by omega)
+  have := (@Nat.pow_lt_pow_eq_pow_mul_le_pow 2 k w (by omega)).mp h
+  rw [Nat.mod_eq_of_lt (by cases b <;> simp [bv_toNat] <;> omega)]
+
+theorem toNat_shiftConcat_lt_of_lt_of_lt_two_pow {x : BitVec w} {b : Bool} {k : Nat}
+    (hk : k < w) (hx : x.toNat < 2 ^ k) :
+    (x.shiftConcat b).toNat < 2 ^ (k + 1) := by
+  rw [toNat_shiftConcat_eq_of_lt_of_lt_two_pow hk hx]
+  apply mul_two_add_lt_two_pow_of_lt_two_pow_of_lt_two hx
+  · cases b <;> decide
+  · omega
+
+/-! ### Division shift subtractor -/
+
+/--
+One round of the division algorithm, that tries to perform a subtract shift.
+Note that this is only called when `r.msb = false`, so we will not overflow.
+-/
+def divSubtractShift (n : BitVec w) (d : BitVec w) (wn : Nat) (qr : DivModState w) :
+    DivModState w :=
+  let r' := shiftConcat qr.r (n.getLsbD (wn - 1)) -- if r ≥ d, then we have a quotient bit.
+  if r' < d
+  then {
+    q := qr.q.shiftConcat false, -- If `r' < d`, then we do not have a quotient bit.
+    r := r'
+  } else {
+    q := qr.q.shiftConcat true, -- If `r' ≥ d`, then we have a quotient bit.
+    r := r' - d -- we subtract to maintain the invariant that `r < d`.
+  }
+
+/-- The value of shifting by `wn - 1` equals shifting by `wn` and grabbing the lsb at `(wn - 1)`. -/
+theorem DivModState.toNat_shiftRight_sub_one_eq
+    (qr : DivModState w) (h : qr.LawfulShiftSubtract wr wn n d):
+    n.toNat >>> (wn - 1) = (n.toNat >>> wn) * 2 + (n.getLsbD (wn - 1)).toNat := by
+  have hn := shiftRight_sub_one_eq_shiftConcat_getLsb_of_lt (n := n) (wn := wn) h.hwn_lt
+  obtain hn : (n >>> (wn - 1)).toNat = ((n >>> wn).shiftConcat (n.getLsbD (wn - 1))).toNat := by
+    simp [hn]
+  simp only [toNat_ushiftRight] at hn
+  rw [toNat_shiftConcat_eq_of_lt_of_lt_two_pow (k := w - wn)] at hn
+  · rw [hn]
+    rw [toNat_ushiftRight]
+  · have := h.hwn_lt
+    have := h.hw
+    omega
+  · apply BitVec.toNat_ushiftRight_lt
+    have := h.hwrn
+    omega
+
+/--
+This is used when proving the correctness of the divison algorithm,
+where we know that `r < d`.
+We then want to show that `((r.shiftConcat b) - d) < d` as the loop invariant.
+In arithmethic, this is the same as showing that
+`r * 2 + 1 - d < d`, which this theorem establishes.
+-/
+private theorem two_mul_add_sub_lt_of_lt_of_lt_two (h : a < x) (hy : y < 2) :
+    2 * a + y - x < x := by omega
+
+/-- We show that the output of `divSubtractShift` is lawful, which tells us that it
+obeys the division equation. -/
+def divSubtractShiftProof (qr : DivModState w) (h : qr.LawfulShiftSubtract  wr wn n d) :
+    DivModState.Lawful w (wr + 1) (wn - 1) n d (divSubtractShift n d wn qr) := by
+  simp only [divSubtractShift, decide_eq_true_eq]
+  -- We add these hypotheses for `omega` to find them later.
+  have ⟨⟨hrwn, hd, hrd, hr, hn, hrnd⟩, hwn_lt⟩ := h
+  have : d.toNat * (qr.q.toNat * 2) = d.toNat * qr.q.toNat * 2 := by rw [Nat.mul_assoc]
+  by_cases rltd : shiftConcat qr.r (n.getLsbD (wn - 1)) < d
+  · simp only [rltd, ↓reduceIte]
+    constructor <;> try bv_omega
+    case pos.hrWidth => apply toNat_shiftConcat_lt_of_lt_of_lt_two_pow <;> omega
+    case pos.hqWidth => apply toNat_shiftConcat_lt_of_lt_of_lt_two_pow <;> omega
+    case pos.hdiv =>
+      simp [qr.toNat_shiftRight_sub_one_eq h, h.hdiv, this,
+        toNat_shiftConcat_eq_of_lt_of_lt_two_pow (qr.wr_lt_w h) h.hrWidth,
+        toNat_shiftConcat_eq_of_lt_of_lt_two_pow (qr.wr_lt_w h) h.hqWidth]
+      omega
+  · simp only [rltd, ↓reduceIte]
+    constructor <;> try bv_omega
+    case neg.hrLtDivisor =>
+      simp only [lt_def, Nat.not_lt] at rltd
+      rw [BitVec.toNat_sub_of_le rltd,
+        toNat_shiftConcat_eq_of_lt_of_lt_two_pow (hk := qr.wr_lt_w h) (hx := h.hrWidth),
+        Nat.mul_comm]
+      apply two_mul_add_sub_lt_of_lt_of_lt_two <;> bv_omega
+    case neg.hrWidth =>
+      simp only
+      have hdr' : d ≤ (qr.r.shiftConcat (n.getLsbD (wn - 1))) :=
+        BitVec.le_iff_not_lt.mp rltd
+      have hr' : ((qr.r.shiftConcat (n.getLsbD (wn - 1)))).toNat < 2 ^ (wr + 1) := by
+        apply toNat_shiftConcat_lt_of_lt_of_lt_two_pow <;> bv_omega
+      rw [BitVec.toNat_sub_of_le hdr']
+      omega
+    case neg.hqWidth =>
+      apply toNat_shiftConcat_lt_of_lt_of_lt_two_pow <;> omega
+    case neg.hdiv =>
+      have rltd' := (BitVec.le_iff_not_lt.mp rltd)
+      simp only [qr.toNat_shiftRight_sub_one_eq h,
+        BitVec.toNat_sub_of_le rltd',
+        toNat_shiftConcat_eq_of_lt_of_lt_two_pow (qr.wr_lt_w h) h.hrWidth]
+      simp only [BitVec.le_def,
+        toNat_shiftConcat_eq_of_lt_of_lt_two_pow (qr.wr_lt_w h) h.hrWidth] at rltd'
+      simp only [toNat_shiftConcat_eq_of_lt_of_lt_two_pow (qr.wr_lt_w h) h.hqWidth, h.hdiv, Nat.mul_add]
+      bv_omega
+
+/-! ### Core division algorithm circuit -/
+
+/-- A recursive definition of division for bitblasting, in terms of a shift-subtraction circuit. -/
+def divRec (w wr wn : Nat) (n d : BitVec w) (qr : DivModState w) :
+    DivModState w :=
+  match wn with
+  | 0 => qr
+  | wn + 1 =>
+    divRec w (wr + 1) wn n d <| divSubtractShift n d (wn + 1) qr
+
+@[simp]
+theorem divRec_zero (qr : DivModState w) :
+  divRec w w 0 n d qr  = qr := rfl
+
+@[simp]
+theorem divRec_succ (wn : Nat) (qr : DivModState w) :
+    divRec w wr (wn + 1) n d qr =
+      divRec w (wr + 1) wn n d
+        (divSubtractShift n d (wn + 1) qr) := rfl
+
+theorem divRec_correct {n d : BitVec w} (qr : DivModState w)
+  (h : DivModState.Lawful w wr wn n d qr) : DivModState.Lawful w w 0 n d (divRec w wr wn n d qr) := by
+  induction wn generalizing wr qr
+  case zero =>
+    unfold divRec
+    simp [← h.hwrn, h]
+  case succ wn' ih =>
+    simp only [divRec]
+    apply ih
+    apply divSubtractShiftProof (w := w)
+      (wr := wr)
+      (wn := wn' + 1)
+    exact h.toLawfulShiftSubtract
+
+/-- The result of `udiv` agrees with the result of the division recurrence. -/
+theorem udiv_eq_divRec (hd : 0#w < d) :
+    let out := divRec w 0 w n d (DivModState.init w)
+    n.udiv d = out.q := by
+  have := DivModState.Lawful.init w n d hd
+  have := divRec_correct (DivModState.init w) this
+  apply DivModState.udiv_eq_of_lawful_zero this
+
+/-- The result of `umod` agrees with the result of the division recurrence. -/
+theorem umod_eq_divRec (hd : 0#w < d) :
+    let out := divRec w 0 w n d (DivModState.init w)
+    n.umod d = out.r := by
+  have := DivModState.Lawful.init w n d hd
+  have := divRec_correct (DivModState.init w) this
+  apply DivModState.umod_eq_of_lawful_zero this
+
+@[simp]
+theorem divRec_succ' (wn : Nat) (qr : DivModState w) :
+    divRec w wr (wn + 1) n d qr =
+    let r' := shiftConcat qr.r (n.getLsbD wn)
+    let input : DivModState w :=
+      if r' < d then ⟨qr.q.shiftConcat false, r'⟩ else ⟨qr.q.shiftConcat true, r' - d⟩
+    divRec w (wr + 1) wn n d input := by
+  simp [divRec_succ, divSubtractShift]
+
 /- ### Arithmetic shift right (sshiftRight) recurrence -/
 
 /--
